Auto/Embedding/Lift.lean
@@ -197,6 +197,21 @@ def bvrotateLeftLift.{u} (w : Nat) (x : GLift.{1, u} (Std.BitVec w)) (n : GLift.
 def bvrotateRightLift.{u} (w : Nat) (x : GLift.{1, u} (Std.BitVec w)) (n : GLift.{1, u} Nat) : GLift.{1, u} (Std.BitVec w) :=
   GLift.up (Std.BitVec.rotateRight x.down n.down)
 
+def bvsmtshlLift.{u} (n : Nat) (a : GLift.{1, u} (Std.BitVec n)) (s : GLift.{1, u} (Std.BitVec n)) : GLift.{1, u} (Std.BitVec n) :=
+  GLift.up (Std.BitVec.shiftLeft a.down s.down.toNat)
+
+def bvsmtlshrLift.{u} (n : Nat) (a : GLift.{1, u} (Std.BitVec n)) (s : GLift.{1, u} (Std.BitVec n)) : GLift.{1, u} (Std.BitVec n) :=
+  GLift.up (Std.BitVec.ushiftRight a.down s.down.toNat)
+
+def bvsmtashrLift.{u} (n : Nat) (a : GLift.{1, u} (Std.BitVec n)) (s : GLift.{1, u} (Std.BitVec n)) : GLift.{1, u} (Std.BitVec n) :=
+  GLift.up (Std.BitVec.sshiftRight a.down s.down.toNat)
+
+def bvsmtrotateLeftLift.{u} (w : Nat) (x : GLift.{1, u} (Std.BitVec w)) (n : GLift.{1, u} (Std.BitVec n)) : GLift.{1, u} (Std.BitVec w) :=
+  GLift.up (Std.BitVec.rotateLeft x.down n.down.toNat)
+
+def bvsmtrotateRightLift.{u} (w : Nat) (x : GLift.{1, u} (Std.BitVec w)) (n : GLift.{1, u} (Std.BitVec n)) : GLift.{1, u} (Std.BitVec w) :=
+  GLift.up (Std.BitVec.rotateRight x.down n.down.toNat)
+
 def bvappendLift.{u} (n m : Nat) (x : GLift.{1, u} (Std.BitVec n)) (y : GLift.{1, u} (Std.BitVec m)) : GLift.{1, u} (Std.BitVec (Nat.add n m)) :=
   GLift.up (Std.BitVec.append x.down y.down)
 
